more dump

code/theories/BasicAst.v
@@ -4,3 +4,10 @@ Axiom base : Set.
 Axiom eqb_base : base -> base -> bool.
 Axiom eqb_base_refl : forall b, eqb_base b b = true.
 Axiom eqb_base_sound : forall b b', eqb_base b b' = true -> b = b'.
+
+Inductive polarity := | pos | neg.
+Definition negp (p : polarity) := if p then neg else pos.
+Lemma negp_inv p : negp (negp p) = p.
+Proof.
+  now destruct p.
+Qed.
