code/theories/Utils.v
@@ -1,5 +1,43 @@
-From Stdlib Require Import Morphisms List CRelationClasses.
+From Stdlib Require Import Morphisms List RelationClasses.
 From smpl Require Import Smpl.
+
+#[export] Set Structural Injection.
+#[export] Add Search Blacklist "_ind" "_sind" "_rec" "_rect".
+#[export] Set Default Goal Selector "!".
+
+(** ** Subtypes *)
+
+Definition incl {A : Type} : (A -> Prop) -> (A -> Prop) -> Prop :=
+  fun P Q => forall x, P x -> Q x.
+
+Notation "P ⊆ Q" := (incl P Q) (at level 90).
+
+Definition inter {A : Type} : (A -> Prop) -> (A -> Prop) -> (A -> Prop) :=
+  fun P Q x => P x /\ Q x.
+
+Notation "P ∩ Q" := (inter P Q) (at level 80).
+
+Arguments inter _ _ _ _/.
+
+Definition union {A : Type} : (A -> Prop) -> (A -> Prop) -> (A -> Prop) :=
+  fun P Q x => P x \/ Q x.
+
+Notation "P ∪ Q" := (union P Q) (at level 85).
+
+Arguments union _ _ _ _/.
+
+Definition empty {A : Type} : A -> Prop := fun _ => False.
+
+Notation "∅" := empty.
+
+Definition sing {A : Type} (a : A) : A -> Prop := fun x => x = a.
+
+Arguments sing _ _ _/.
+
+(** ** Notations *)
+
+Notation "`=1`" := (pointwise_relation _ Logic.eq) (at level 80).
+Infix "=1" := (pointwise_relation _ Logic.eq) (at level 70).
 
 (** ** Tactics *)
 
@@ -16,6 +54,14 @@ Ltac prod_splitter :=
   | |- _ /\ _ => split
   end.
 
+(** An arbitrary reflexive relation relates equal terms *)
+Lemma ereflexivity {A} {R} `{Reflexive A R} {x y} :
+  x = y -> R x y.
+Proof.
+  intros ->.
+  reflexivity.
+Qed.
+
 (** A general refolding tactic to recover lost typeclasses
   (due for instance to the cbn or constructor tactics).
   Updated on the fly using the Smpl plugin. *)
@@ -28,3 +74,13 @@ Tactic Notation "constructor" := core_constructor ; refold.
 
 Ltac core_econstructor := econstructor.
 Tactic Notation "econstructor" := core_econstructor ; refold.
+
+(** Tactics used to create good induction principles using Scheme *)
+
+Ltac remove_steps t :=
+  lazymatch t with
+  | _ -> ?T => remove_steps T
+  | forall x : ?Hyp, @?T x => constr:(fun  x : Hyp => ltac:(
+      let T' := ltac:(eval hnf in (T x)) in let T'' := remove_steps T' in exact T''))
+  | ?t' => t'
+  end.
