code/theories/Bidir.v
@@ -1,0 +1,63 @@
+From Interpolation Require Import Utils Syntax Typing.
+From Stdlib Require Import Relations Arith Lia Bool List.
+
+Reserved Notation "Γ '|-' t ▹ T"
+  (at level 101, t at level 59).
+Reserved Notation "Γ '|-' t ◃ T"
+  (at level 101, t at level 59).
+
+Unset Elimination Schemes.
+
+Inductive check : context -> type -> term -> Prop :=
+| C_Star Γ : (Γ |- tStar ◃ TUnit)
+
+| C_Abs Γ (A B : type) t :
+  (Γ ,,, A |- t ◃ B) ->
+  Γ |- tLam t ◃ TFun A B
+
+| C_Pair Γ A B a b :
+  (Γ |- a ◃ A) ->
+  (Γ |- b ◃ B) ->
+  (Γ |- tPair a b ◃ TProd A B)
+
+| C_inf Γ A A' t :
+  (Γ |- t ▹ A') ->
+  A' = A ->
+  (Γ |- t ◃ A)
+
+with infer : context -> type -> term -> Prop :=
+| I_Var Γ n T :
+  in_context n Γ T ->
+  Γ |- tVar n ▹ T
+
+| I_App Γ A B f u :
+  (Γ |- f ▹ TFun A B) ->
+  (Γ |- u ◃ A) ->
+  Γ |- tApp f u ▹ B
+
+| I_Fst Γ A B t :
+  (Γ |- t ▹ TProd A B) ->
+  (Γ |- tFst t ▹ A)
+
+| I_Snd Γ A B t :
+  (Γ |- t ▹ TProd A B) ->
+  (Γ |- tSnd t ▹ B)
+
+where "Γ '|-' t ▹ T" := (infer Γ T t) (Γ in scope context_scope)
+and "Γ '|-' t ◃ T" := (check Γ T t) (Γ in scope context_scope).
+
+Hint Constructors check infer : core.
+
+Scheme 
+Minimality for check Sort Prop with
+Minimality for infer Sort Prop.
+
+Combined Scheme bidir_ind from check_ind, infer_ind.
+
+Definition bidir_concl :=
+ltac:(
+let t := type of bidir_ind in
+let t' := remove_steps t in
+exact t').
+
+Arguments bidir_concl Pcheck Pinf : rename.
