code/theories/Interpolation.v
@@ -1,0 +1,222 @@
+From Interpolation Require Import Utils Syntax Reduction Typing Bidir.
+From Stdlib Require Import Relations Arith Lia Bool List RelationClasses.
+
+(** ** Primitives for context splitting *)
+
+Inductive side : Set := | source | target.
+
+Inductive split : context -> context -> context -> Set :=
+  | split_emp : split ε ε ε
+  | split_s {Γ Γs Γt A} : split Γ Γs Γt -> split (Γ,,,A) (Γs,,,A) Γt
+  | split_t {Γ Γs Γt A} : split Γ Γs Γt -> split (Γ,,,A) Γs (Γt,,,A).
+
+Fixpoint find_side {Γ Γs Γt} (n : nat) (s : split Γ Γs Γt) : option side :=
+  match n, s with
+  | _, split_emp => None
+  | 0, split_s _ => Some source
+  | 0, split_t _ => Some target
+  | S n', split_s s' | S n', split_t s' => find_side n' s'
+  end.
+
+Lemma in_context_find {Γ Γs Γt} (n : nat) (s : split Γ Γs Γt) T :
+  in_context n Γ T ->
+  find_side n s = None ->
+  False.
+Proof.
+  induction s in n |- * ; [|destruct n | destruct n] ; cbn.
+  - intros ; now eapply var_empty.
+  - congruence.
+  - intros Hin ?%IHs.
+    1: easy.
+    exact Hin.
+  - congruence.
+  - intros Hin ?%IHs.
+    1: easy.
+    exact Hin.
+Qed.
+
+Fixpoint flip_split {Γ Γs Γt} (s : split Γ Γs Γt) : split Γ Γt Γs :=
+  match s with
+  | split_emp => split_emp
+  | split_s s => split_t (flip_split s)
+  | split_t s => split_s (flip_split s)
+  end. 
+
+Fixpoint split_ren_s {Γ Γs Γt} (s : split Γ Γs Γt) : ren :=
+  match s with
+  | split_emp => id
+  | split_s s' => up_ren (split_ren_s s')
+  | split_t s' => (split_ren_s s') >> ↑
+  end.
+
+Fixpoint split_ren_t {Γ Γs Γt} (s : split Γ Γs Γt) : ren :=
+  match s with
+  | split_emp => id
+  | split_t s' => up_ren (split_ren_t s')
+  | split_s s' => (split_ren_t s') >> ↑
+  end.
+
+Lemma split_ren_s_ty {Γ Γs Γt} (s : split Γ Γs Γt) :
+  ren_has_type Γ Γs (split_ren_s s).
+Proof.
+  induction s ; cbn.
+  - apply id_ren_has_type.
+  - now apply ren_lift_has_type.
+  - eapply ren_comp_has_type ; tea.
+    apply shift_has_type.
+Qed.
+
+Lemma split_ren_t_ty {Γ Γs Γt} (s : split Γ Γs Γt) :
+  ren_has_type Γ Γt (split_ren_t s).
+Proof.
+  induction s ; cbn.
+  - apply id_ren_has_type.
+  - eapply ren_comp_has_type ; tea.
+    apply shift_has_type.
+  - now apply ren_lift_has_type.
+Qed.
+
+(** ** Atoms of a type/context *)
+
+Fixpoint atoms_ty (p : polarity) (A : type) {struct A} : base -> Prop :=
+  match A with
+  | TBase b => if p then (sing b) else ∅
+  | TUnit => ∅
+  | TFun A B => atoms_ty (negp p) A ∪ atoms_ty p B
+  | TProd A B => atoms_ty p A ∪ atoms_ty p B
+  end.
+
+Fixpoint atoms_ctx (p : polarity) (Γ : context) : base -> Prop :=
+  match Γ with
+  | nil => ∅
+  | cons A Γ => atoms_ctx p Γ ∪ (atoms_ty p A)
+  end.
+
+Section Interpolation.
+
+(** With the splitting of the context given by Γs and Γt and the type A,
+  I is a valid interpolating type. *)
+Definition interpolate_ty Γs Γt A M :=
+  forall p, atoms_ty p M ⊆ (atoms_ctx p Γs) ∩ (atoms_ctx (negp p) Γt ∪ atoms_ty p A).
+
+Definition interpolate_tm {Γ Γs Γt} (s : split Γ Γs Γt) M A t l r :=
+  (Γs |- l :: M) /\ (Γt ,,, M |- r :: A) /\
+  r⟨up_ren (split_ren_t s)⟩[l⟨split_ren_s s⟩..] -->* t.
+
+Let Pcheck Γ T t := forall Γs Γt (s : split Γ Γs Γt),
+  exists M l r,
+    (forall p, atoms_ty p M ⊆ (atoms_ctx p Γs) ∩ (atoms_ctx (negp p) Γt ∪ atoms_ty p T)) /\ interpolate_tm s M T t l r.
+
+Let Pinf Γ T t := forall Γs Γt (s : split Γ Γs Γt),
+  (
+    (forall p, atoms_ty p T ⊆ atoms_ctx (negp p) Γt) /\
+    (exists M l r, 
+      (forall p, atoms_ty p M ⊆ (atoms_ctx p Γs) ∩ (atoms_ctx (negp p) Γt)) /\
+      interpolate_tm s M T t l r)
+  ) \/ (
+    (forall p, atoms_ty p T ⊆ atoms_ctx p Γs) /\
+    (exists M l r, 
+      (forall p, atoms_ty p M ⊆ (atoms_ctx (negp p) Γs) ∩ (atoms_ctx p Γt)) /\
+      interpolate_tm (flip_split s) M T t l r)
+  ).
+
+Definition swap_var : ren :=
+  fun n => match n with
+  | 0 => 1
+  | 1 => 0
+  | n => n
+  end.
+
+Lemma swap_var_ty : forall Γ (A B : type),
+  ren_has_type ((Γ,,,A),,,B) ((Γ,,,B),,,A) swap_var.
+Proof.
+  intros Γ A B i T Hin.
+  destruct i as [|[|i]] ; cbn in *.
+  all: exact Hin.
+Qed.
+
+(* Hypothesis swap_var_eq : forall t u, t [u..] = t [swap_var] [⇑ (u..)]. *)
+
+Theorem interpolation : bidir_concl Pcheck Pinf.
+Proof.
+  apply bidir_ind.
+  - intros Γ Γs Γt s.
+    exists TUnit, tStar, tStar.
+    split.
+    + intros ; cbn.
+      intros ? [].
+    + red.
+      prod_splitter.
+      all: solve [constructor].
+  - intros Γ A B t _ IH Γs Γt s.
+    destruct (IH Γs (Γt,,,A) (split_t s)) as (M&l&r&HM&Ht).
+    exists M, l, (tLam (r⟨swap_var⟩)).
+    split.
+    (* the good-looking proof would do setoid rewriting with subset equivalence… *)
+    + intros p b Hb.
+      specialize (HM p b Hb).
+      now cbn in *.
+    + unfold interpolate_tm in * ; cbn in *.
+      destruct Ht as (?&?&e).
+      prod_splitter.
+      1: easy.
+      * constructor.
+        eapply ren_typing ; [|eassumption].
+        apply swap_var_ty.
+      * apply R_Lam_cong.
+        etransitivity ; tea.
+        apply ereflexivity.
+        substify.
+        asimpl.
+        apply ext_term.
+        intros [|[|]] ; reflexivity.
+  - intros Γ A B t t' _ IHA _ IHB Γs Γt s.
+    destruct (IHA Γs Γt s) as (M & l & r & HM & Ht).
+    destruct (IHB Γs Γt s) as (M' & l' & r' & HM' & Ht').
+    exists (TProd M M'), (tPair l l'),
+      (tPair (r[(tFst (tVar 0)).: (↑ >> tVar)]) (r'[(tSnd (tVar 0)) .: (↑ >> tVar)])).
+    split.
+    + intros p b [Hb|Hb'].
+      1: specialize (HM p b Hb).
+      2: specialize (HM' p b Hb').
+      all: now cbn in *.
+    + unfold interpolate_tm in * ; cbn in *.
+      prod_splitter.
+      1: now constructor.
+      * constructor.
+        all: eapply subst_typing ; [|easy].
+        all: eapply subst_cons_has_type ; [apply ren_subst_has_type, shift_has_type|..].
+        all: repeat econstructor.
+      * apply R_Pair_cong.
+        all: etransitivity ; [|easy].
+        all: admit.
+  - intros * _ IH -> ?? s.
+    destruct (IH _ _ s) as [[? (M&l&r&[HM ?])]|[Hat (M&l&r&[HM ?])]] ; tea.
+    + exists M, l, r ; split.
+      2: easy.
+      intros p b [?%HM Hb]%dup ; cbn in * ; easy.
+    + exists (TFun M A), (tLam r), (tApp (tVar 0) l⟨↑⟩).
+      split.
+      * intros p b [[HΓ%HM Hb]%dup| HA] ; cbn in *.
+        1: rewrite negp_inv in HΓ ; easy.
+        split ; [|easy].
+        now apply Hat.
+      * unfold interpolate_tm in *.
+        prod_splitter.
+        1: now econstructor.
+        1: econstructor ; [easy|..] ; eapply ren_typing ; [|easy] ; now apply shift_has_type.
+        cbn.
+        etransitivity.
+        1: constructor ; apply ST_Beta.
+        admit.
+  - intros ? n T Hin ?? s.
+    destruct (find_side n s) as [[]|] eqn:e.
+    3: exfalso ; now eauto using in_context_find.
+    + admit.
+    + admit.
+  - admit.
+  - admit.
+  - admit.
+Admitted.
+
+End Interpolation.
