code/theories/Reduction.v
@@ -1,0 +1,81 @@
+From Interpolation Require Import Utils Syntax.
+From Stdlib Require Import Relations Arith Lia Bool List RelationClasses.
+
+Import ListNotations.
+
+(** ** Reduction *)
+
+Reserved Notation "t '-->' t'" (at level 40).
+
+Inductive step : term -> term -> Prop :=
+  | ST_Beta t1 v2 :
+        tApp (tLam t1) v2 --> t1[v2..]
+  | ST_App_l t1 t1' t2 :
+         t1 --> t1' ->
+         tApp t1 t2 --> tApp t1' t2
+  | ST_App_r t1 t2 t2' :
+         t2 --> t2' ->
+         tApp t1 t2 --> tApp t1 t2'
+  | ST_Lam t t' :
+    t --> t' ->
+    tLam t --> tLam t'
+  | ST_Fst t t' : tFst (tPair t t') --> t
+  | ST_Snd t t' : tSnd (tPair t t') --> t'
+  | ST_Proj b t t' :
+         t --> t' ->
+         tProj b t --> tProj b t'
+  | ST_Pair_l t1 t1' t2 :
+         t1 --> t1' ->
+         tPair t1 t2 --> tPair t1' t2
+  | ST_Par_r t1 t2 t2' :
+         t2 --> t2' ->
+         tPair t1 t2 --> tPair t1 t2'
+
+where "t '-->' t'" := (step t t').
+
+Hint Constructors step : core.
+
+Notation multistep := (clos_refl_trans term step).
+Notation "t1 '-->*' t2" := (multistep t1 t2) (at level 40).
+
+Instance red_po : PreOrder multistep.
+Proof.
+  constructor.
+  all: now econstructor.
+Qed.
+
+Lemma R_App_cong f f' u u':
+  f -->* f' ->
+  u -->* u' ->
+  tApp f u -->* tApp f' u'.
+Proof.
+  intros Hf Hu.
+  induction Hf using clos_refl_trans_ind_left ; eauto using rt_refl, rt_step, rt_trans.
+  induction Hu using clos_refl_trans_ind_left ; eauto using rt_refl, rt_step, rt_trans.
+Qed.
+
+Lemma R_Lam_cong t t':
+  t -->* t' ->
+  tLam t -->* tLam t'.
+Proof.
+  intros Ht.
+  induction Ht using clos_refl_trans_ind_left ; eauto using rt_refl, rt_step, rt_trans.
+Qed.
+
+Lemma R_Proj_cong b t t' :
+  t -->* t' ->
+  tProj b t -->* tProj b t'.
+Proof.
+  intros Hred.
+  induction Hred using clos_refl_trans_ind_left ; eauto using rt_refl, rt_step, rt_trans.
+Qed.
+
+Lemma R_Pair_cong p p' q q':
+  p -->* p' ->
+  q -->* q' ->
+  tPair p q -->* tPair p' q'.
+Proof.
+  intros Hp Hq.
+  induction Hp using clos_refl_trans_ind_left ; eauto using rt_refl, rt_step, rt_trans.
+  induction Hq using clos_refl_trans_ind_left ; eauto using rt_refl, rt_step, rt_trans.
+Qed.
